Add u32/u64 SSZ endian models, specs, and proofs

formal/model/ssz_endian_model.v
@@ -7,6 +7,10 @@ Local Open Scope Z_scope.
 Definition byte_modulus : Z := 2 ^ 8.
 Definition uint16_modulus : Z := 2 ^ 16.
 Definition uint16_max : Z := uint16_modulus - 1.
+Definition uint32_modulus : Z := 2 ^ 32.
+Definition uint32_max : Z := uint32_modulus - 1.
+Definition uint64_modulus : Z := 2 ^ 64.
+Definition uint64_max : Z := uint64_modulus - 1.
 
 Definition ssz_u16_le_byte0 (value : Z) : byte :=
   Byte.repr (value mod byte_modulus).
@@ -24,8 +28,90 @@ Definition ssz_u16_le_decode (bytes : list byte) : Z :=
   | _ => 0
   end.
 
+Definition ssz_u32_le_byte0 (value : Z) : byte :=
+  Byte.repr (value mod byte_modulus).
+
+Definition ssz_u32_le_byte1 (value : Z) : byte :=
+  Byte.repr ((value / byte_modulus) mod byte_modulus).
+
+Definition ssz_u32_le_byte2 (value : Z) : byte :=
+  Byte.repr ((value / byte_modulus ^ 2) mod byte_modulus).
+
+Definition ssz_u32_le_byte3 (value : Z) : byte :=
+  Byte.repr ((value / byte_modulus ^ 3) mod byte_modulus).
+
+Definition ssz_u32_le_bytes (value : Z) : list byte :=
+  [ssz_u32_le_byte0 value; ssz_u32_le_byte1 value;
+   ssz_u32_le_byte2 value; ssz_u32_le_byte3 value].
+
+Definition ssz_u32_le_decode (bytes : list byte) : Z :=
+  match bytes with
+  | [byte0; byte1; byte2; byte3] =>
+      Byte.unsigned byte0 +
+      byte_modulus * Byte.unsigned byte1 +
+      byte_modulus ^ 2 * Byte.unsigned byte2 +
+      byte_modulus ^ 3 * Byte.unsigned byte3
+  | _ => 0
+  end.
+
+Definition ssz_u64_le_byte0 (value : Z) : byte :=
+  Byte.repr (value mod byte_modulus).
+
+Definition ssz_u64_le_byte1 (value : Z) : byte :=
+  Byte.repr ((value / byte_modulus) mod byte_modulus).
+
+Definition ssz_u64_le_byte2 (value : Z) : byte :=
+  Byte.repr ((value / byte_modulus ^ 2) mod byte_modulus).
+
+Definition ssz_u64_le_byte3 (value : Z) : byte :=
+  Byte.repr ((value / byte_modulus ^ 3) mod byte_modulus).
+
+Definition ssz_u64_le_byte4 (value : Z) : byte :=
+  Byte.repr ((value / byte_modulus ^ 4) mod byte_modulus).
+
+Definition ssz_u64_le_byte5 (value : Z) : byte :=
+  Byte.repr ((value / byte_modulus ^ 5) mod byte_modulus).
+
+Definition ssz_u64_le_byte6 (value : Z) : byte :=
+  Byte.repr ((value / byte_modulus ^ 6) mod byte_modulus).
+
+Definition ssz_u64_le_byte7 (value : Z) : byte :=
+  Byte.repr ((value / byte_modulus ^ 7) mod byte_modulus).
+
+Definition ssz_u64_le_bytes (value : Z) : list byte :=
+  [ssz_u64_le_byte0 value; ssz_u64_le_byte1 value;
+   ssz_u64_le_byte2 value; ssz_u64_le_byte3 value;
+   ssz_u64_le_byte4 value; ssz_u64_le_byte5 value;
+   ssz_u64_le_byte6 value; ssz_u64_le_byte7 value].
+
+Definition ssz_u64_le_decode (bytes : list byte) : Z :=
+  match bytes with
+  | [byte0; byte1; byte2; byte3; byte4; byte5; byte6; byte7] =>
+      Byte.unsigned byte0 +
+      byte_modulus * Byte.unsigned byte1 +
+      byte_modulus ^ 2 * Byte.unsigned byte2 +
+      byte_modulus ^ 3 * Byte.unsigned byte3 +
+      byte_modulus ^ 4 * Byte.unsigned byte4 +
+      byte_modulus ^ 5 * Byte.unsigned byte5 +
+      byte_modulus ^ 6 * Byte.unsigned byte6 +
+      byte_modulus ^ 7 * Byte.unsigned byte7
+  | _ => 0
+  end.
+
 Lemma ssz_u16_le_bytes_length :
   forall value, Zlength (ssz_u16_le_bytes value) = 2.
+Proof.
+  intros; reflexivity.
+Qed.
+
+Lemma ssz_u32_le_bytes_length :
+  forall value, Zlength (ssz_u32_le_bytes value) = 4.
+Proof.
+  intros; reflexivity.
+Qed.
+
+Lemma ssz_u64_le_bytes_length :
+  forall value, Zlength (ssz_u64_le_bytes value) = 8.
 Proof.
   intros; reflexivity.
 Qed.
@@ -51,6 +137,44 @@ Proof.
   change (2 ^ 16) with 65536.
   pose proof (Byte.unsigned_range_2 byte0).
   pose proof (Byte.unsigned_range_2 byte1).
+  change Byte.max_unsigned with 255 in *.
+  lia.
+Qed.
+
+Lemma ssz_u32_le_decode_range :
+  forall byte0 byte1 byte2 byte3,
+    0 <= ssz_u32_le_decode [byte0; byte1; byte2; byte3] <= uint32_max.
+Proof.
+  intros byte0 byte1 byte2 byte3.
+  unfold ssz_u32_le_decode, byte_modulus, uint32_max, uint32_modulus.
+  change (2 ^ 8) with 256.
+  change (2 ^ 32) with 4294967296.
+  pose proof (Byte.unsigned_range_2 byte0).
+  pose proof (Byte.unsigned_range_2 byte1).
+  pose proof (Byte.unsigned_range_2 byte2).
+  pose proof (Byte.unsigned_range_2 byte3).
+  change Byte.max_unsigned with 255 in *.
+  lia.
+Qed.
+
+Lemma ssz_u64_le_decode_range :
+  forall byte0 byte1 byte2 byte3 byte4 byte5 byte6 byte7,
+    0 <= ssz_u64_le_decode
+      [byte0; byte1; byte2; byte3; byte4; byte5; byte6; byte7] <=
+    uint64_max.
+Proof.
+  intros byte0 byte1 byte2 byte3 byte4 byte5 byte6 byte7.
+  unfold ssz_u64_le_decode, byte_modulus, uint64_max, uint64_modulus.
+  change (2 ^ 8) with 256.
+  change (2 ^ 64) with 18446744073709551616.
+  pose proof (Byte.unsigned_range_2 byte0).
+  pose proof (Byte.unsigned_range_2 byte1).
+  pose proof (Byte.unsigned_range_2 byte2).
+  pose proof (Byte.unsigned_range_2 byte3).
+  pose proof (Byte.unsigned_range_2 byte4).
+  pose proof (Byte.unsigned_range_2 byte5).
+  pose proof (Byte.unsigned_range_2 byte6).
+  pose proof (Byte.unsigned_range_2 byte7).
   change Byte.max_unsigned with 255 in *.
   lia.
 Qed.
@@ -111,6 +235,345 @@ Proof.
   apply Hneq.
   pose proof (f_equal ssz_u16_le_decode Hbytes) as Hdecoded.
   rewrite !ssz_u16_le_decode_encode_roundtrip in Hdecoded by assumption.
+  exact Hdecoded.
+Qed.
+
+Lemma ssz_u32_le_decode_encode_roundtrip :
+  forall value,
+    0 <= value <= uint32_max ->
+    ssz_u32_le_decode (ssz_u32_le_bytes value) = value.
+Proof.
+  intros value Hrange.
+  unfold ssz_u32_le_decode, ssz_u32_le_bytes,
+    ssz_u32_le_byte0, ssz_u32_le_byte1,
+    ssz_u32_le_byte2, ssz_u32_le_byte3.
+  assert (Hbyte0 : 0 <= value mod byte_modulus <= Byte.max_unsigned).
+  {
+    unfold byte_modulus.
+    change (2 ^ 8) with 256.
+    change Byte.max_unsigned with 255.
+    pose proof (Z.mod_pos_bound value 256 ltac:(lia)).
+    lia.
+  }
+  assert (Hbyte1 :
+    0 <= (value / byte_modulus) mod byte_modulus <= Byte.max_unsigned).
+  {
+    unfold byte_modulus.
+    change (2 ^ 8) with 256.
+    change Byte.max_unsigned with 255.
+    pose proof (Z.mod_pos_bound (value / 256) 256 ltac:(lia)).
+    lia.
+  }
+  assert (Hbyte2 :
+    0 <= (value / byte_modulus ^ 2) mod byte_modulus <= Byte.max_unsigned).
+  {
+    unfold byte_modulus.
+    change (2 ^ 8) with 256.
+    change (256 ^ 2) with 65536.
+    change Byte.max_unsigned with 255.
+    pose proof (Z.mod_pos_bound (value / 65536) 256 ltac:(lia)).
+    lia.
+  }
+  assert (Hbyte3 :
+    0 <= (value / byte_modulus ^ 3) mod byte_modulus <= Byte.max_unsigned).
+  {
+    unfold byte_modulus.
+    change (2 ^ 8) with 256.
+    change (256 ^ 3) with 16777216.
+    change Byte.max_unsigned with 255.
+    pose proof (Z.mod_pos_bound (value / 16777216) 256 ltac:(lia)).
+    lia.
+  }
+  rewrite Byte.unsigned_repr by exact Hbyte0.
+  rewrite Byte.unsigned_repr by exact Hbyte1.
+  rewrite Byte.unsigned_repr by exact Hbyte2.
+  rewrite Byte.unsigned_repr by exact Hbyte3.
+  unfold byte_modulus.
+  change (2 ^ 8) with 256.
+  change (256 ^ 2) with 65536.
+  change (256 ^ 3) with 16777216.
+  set (q1 := value / 256).
+  set (q2 := value / 65536).
+  set (q3 := value / 16777216).
+  set (r0 := value mod 256).
+  set (r1 := value / 256 mod 256).
+  set (r2 := value / 65536 mod 256).
+  set (r3 := value / 16777216 mod 256).
+  change (r0 + 256 * r1 + 65536 * r2 + 16777216 * r3 = value).
+  assert (Hvalue_lt : value < 4294967296).
+  {
+    unfold uint32_max, uint32_modulus in Hrange.
+    change (2 ^ 32) with 4294967296 in Hrange.
+    lia.
+  }
+  assert (Hstep0 : value = q1 * 256 + r0).
+  {
+    subst q1 r0.
+    pose proof (Z.div_mod value 256 ltac:(lia)) as Hstep.
+    rewrite Z.mul_comm in Hstep.
+    exact Hstep.
+  }
+  assert (Hstep1 : q1 = q2 * 256 + r1).
+  {
+    subst q1 q2 r1.
+    pose proof (Z.div_mod (value / 256) 256 ltac:(lia)) as Hstep.
+    replace (value / 256 / 256) with (value / 65536) in Hstep by
+      (rewrite Z.div_div by lia; reflexivity).
+    lia.
+  }
+  assert (Hstep2 : q2 = q3 * 256 + r2).
+  {
+    subst q2 q3 r2.
+    pose proof (Z.div_mod (value / 65536) 256 ltac:(lia)) as Hstep.
+    replace (value / 65536 / 256) with (value / 16777216) in Hstep by
+      (rewrite Z.div_div by lia; reflexivity).
+    lia.
+  }
+  assert (Hq3 : 0 <= value / 16777216 < 256).
+  {
+    split.
+    - apply Z.div_pos; lia.
+    - apply Z.div_lt_upper_bound; lia.
+  }
+  assert (Hstep3 : r3 = q3).
+  {
+    subst q3 r3.
+    rewrite Z.mod_small; lia.
+  }
+  nia.
+Qed.
+
+Lemma ssz_u32_le_bytes_injective :
+  forall value1 value2,
+    0 <= value1 <= uint32_max ->
+    0 <= value2 <= uint32_max ->
+    value1 <> value2 ->
+    ssz_u32_le_bytes value1 <> ssz_u32_le_bytes value2.
+Proof.
+  intros value1 value2 Hrange1 Hrange2 Hneq Hbytes.
+  apply Hneq.
+  pose proof (f_equal ssz_u32_le_decode Hbytes) as Hdecoded.
+  rewrite !ssz_u32_le_decode_encode_roundtrip in Hdecoded by assumption.
+  exact Hdecoded.
+Qed.
+
+Lemma ssz_u64_le_decode_encode_roundtrip :
+  forall value,
+    0 <= value <= uint64_max ->
+    ssz_u64_le_decode (ssz_u64_le_bytes value) = value.
+Proof.
+  intros value Hrange.
+  unfold ssz_u64_le_decode, ssz_u64_le_bytes,
+    ssz_u64_le_byte0, ssz_u64_le_byte1,
+    ssz_u64_le_byte2, ssz_u64_le_byte3,
+    ssz_u64_le_byte4, ssz_u64_le_byte5,
+    ssz_u64_le_byte6, ssz_u64_le_byte7.
+  assert (Hbyte0 : 0 <= value mod byte_modulus <= Byte.max_unsigned).
+  {
+    unfold byte_modulus.
+    change (2 ^ 8) with 256.
+    change Byte.max_unsigned with 255.
+    pose proof (Z.mod_pos_bound value 256 ltac:(lia)).
+    lia.
+  }
+  assert (Hbyte1 :
+    0 <= (value / byte_modulus) mod byte_modulus <= Byte.max_unsigned).
+  {
+    unfold byte_modulus.
+    change (2 ^ 8) with 256.
+    change Byte.max_unsigned with 255.
+    pose proof (Z.mod_pos_bound (value / 256) 256 ltac:(lia)).
+    lia.
+  }
+  assert (Hbyte2 :
+    0 <= (value / byte_modulus ^ 2) mod byte_modulus <= Byte.max_unsigned).
+  {
+    unfold byte_modulus.
+    change (2 ^ 8) with 256.
+    change (256 ^ 2) with 65536.
+    change Byte.max_unsigned with 255.
+    pose proof (Z.mod_pos_bound (value / 65536) 256 ltac:(lia)).
+    lia.
+  }
+  assert (Hbyte3 :
+    0 <= (value / byte_modulus ^ 3) mod byte_modulus <= Byte.max_unsigned).
+  {
+    unfold byte_modulus.
+    change (2 ^ 8) with 256.
+    change (256 ^ 3) with 16777216.
+    change Byte.max_unsigned with 255.
+    pose proof (Z.mod_pos_bound (value / 16777216) 256 ltac:(lia)).
+    lia.
+  }
+  assert (Hbyte4 :
+    0 <= (value / byte_modulus ^ 4) mod byte_modulus <= Byte.max_unsigned).
+  {
+    unfold byte_modulus.
+    change (2 ^ 8) with 256.
+    change (256 ^ 4) with 4294967296.
+    change Byte.max_unsigned with 255.
+    pose proof (Z.mod_pos_bound (value / 4294967296) 256 ltac:(lia)).
+    lia.
+  }
+  assert (Hbyte5 :
+    0 <= (value / byte_modulus ^ 5) mod byte_modulus <= Byte.max_unsigned).
+  {
+    unfold byte_modulus.
+    change (2 ^ 8) with 256.
+    change (256 ^ 5) with 1099511627776.
+    change Byte.max_unsigned with 255.
+    pose proof (Z.mod_pos_bound (value / 1099511627776) 256 ltac:(lia)).
+    lia.
+  }
+  assert (Hbyte6 :
+    0 <= (value / byte_modulus ^ 6) mod byte_modulus <= Byte.max_unsigned).
+  {
+    unfold byte_modulus.
+    change (2 ^ 8) with 256.
+    change (256 ^ 6) with 281474976710656.
+    change Byte.max_unsigned with 255.
+    pose proof (Z.mod_pos_bound (value / 281474976710656) 256 ltac:(lia)).
+    lia.
+  }
+  assert (Hbyte7 :
+    0 <= (value / byte_modulus ^ 7) mod byte_modulus <= Byte.max_unsigned).
+  {
+    unfold byte_modulus.
+    change (2 ^ 8) with 256.
+    change (256 ^ 7) with 72057594037927936.
+    change Byte.max_unsigned with 255.
+    pose proof (Z.mod_pos_bound (value / 72057594037927936) 256 ltac:(lia)).
+    lia.
+  }
+  rewrite Byte.unsigned_repr by exact Hbyte0.
+  rewrite Byte.unsigned_repr by exact Hbyte1.
+  rewrite Byte.unsigned_repr by exact Hbyte2.
+  rewrite Byte.unsigned_repr by exact Hbyte3.
+  rewrite Byte.unsigned_repr by exact Hbyte4.
+  rewrite Byte.unsigned_repr by exact Hbyte5.
+  rewrite Byte.unsigned_repr by exact Hbyte6.
+  rewrite Byte.unsigned_repr by exact Hbyte7.
+  unfold byte_modulus.
+  change (2 ^ 8) with 256.
+  change (256 ^ 2) with 65536.
+  change (256 ^ 3) with 16777216.
+  change (256 ^ 4) with 4294967296.
+  change (256 ^ 5) with 1099511627776.
+  change (256 ^ 6) with 281474976710656.
+  change (256 ^ 7) with 72057594037927936.
+  set (q1 := value / 256).
+  set (q2 := value / 65536).
+  set (q3 := value / 16777216).
+  set (q4 := value / 4294967296).
+  set (q5 := value / 1099511627776).
+  set (q6 := value / 281474976710656).
+  set (q7 := value / 72057594037927936).
+  set (r0 := value mod 256).
+  set (r1 := value / 256 mod 256).
+  set (r2 := value / 65536 mod 256).
+  set (r3 := value / 16777216 mod 256).
+  set (r4 := value / 4294967296 mod 256).
+  set (r5 := value / 1099511627776 mod 256).
+  set (r6 := value / 281474976710656 mod 256).
+  set (r7 := value / 72057594037927936 mod 256).
+  change
+    (r0 + 256 * r1 + 65536 * r2 + 16777216 * r3 +
+     4294967296 * r4 + 1099511627776 * r5 +
+     281474976710656 * r6 + 72057594037927936 * r7 = value).
+  assert (Hvalue_lt : value < 18446744073709551616).
+  {
+    unfold uint64_max, uint64_modulus in Hrange.
+    change (2 ^ 64) with 18446744073709551616 in Hrange.
+    lia.
+  }
+  assert (Hstep0 : value = q1 * 256 + r0).
+  {
+    subst q1 r0.
+    pose proof (Z.div_mod value 256 ltac:(lia)).
+    lia.
+  }
+  assert (Hstep1 : q1 = q2 * 256 + r1).
+  {
+    subst q1 q2 r1.
+    pose proof (Z.div_mod (value / 256) 256 ltac:(lia)) as Hstep.
+    replace (value / 256 / 256) with (value / 65536) in Hstep by
+      (rewrite Z.div_div by lia; reflexivity).
+    rewrite Z.mul_comm in Hstep.
+    exact Hstep.
+  }
+  assert (Hstep2 : q2 = q3 * 256 + r2).
+  {
+    subst q2 q3 r2.
+    pose proof (Z.div_mod (value / 65536) 256 ltac:(lia)) as Hstep.
+    replace (value / 65536 / 256) with (value / 16777216) in Hstep by
+      (rewrite Z.div_div by lia; reflexivity).
+    rewrite Z.mul_comm in Hstep.
+    exact Hstep.
+  }
+  assert (Hstep3 : q3 = q4 * 256 + r3).
+  {
+    subst q3 q4 r3.
+    pose proof (Z.div_mod (value / 16777216) 256 ltac:(lia)) as Hstep.
+    replace (value / 16777216 / 256) with (value / 4294967296) in Hstep by
+      (rewrite Z.div_div by lia; reflexivity).
+    rewrite Z.mul_comm in Hstep.
+    exact Hstep.
+  }
+  assert (Hstep4 : q4 = q5 * 256 + r4).
+  {
+    subst q4 q5 r4.
+    pose proof (Z.div_mod (value / 4294967296) 256 ltac:(lia)) as Hstep.
+    replace (value / 4294967296 / 256)
+      with (value / 1099511627776) in Hstep by
+      (rewrite Z.div_div by lia; reflexivity).
+    rewrite Z.mul_comm in Hstep.
+    exact Hstep.
+  }
+  assert (Hstep5 : q5 = q6 * 256 + r5).
+  {
+    subst q5 q6 r5.
+    pose proof (Z.div_mod (value / 1099511627776) 256 ltac:(lia)) as Hstep.
+    replace (value / 1099511627776 / 256)
+      with (value / 281474976710656) in Hstep by
+      (rewrite Z.div_div by lia; reflexivity).
+    rewrite Z.mul_comm in Hstep.
+    exact Hstep.
+  }
+  assert (Hstep6 : q6 = q7 * 256 + r6).
+  {
+    subst q6 q7 r6.
+    pose proof (Z.div_mod (value / 281474976710656) 256 ltac:(lia)) as Hstep.
+    replace (value / 281474976710656 / 256)
+      with (value / 72057594037927936) in Hstep by
+      (rewrite Z.div_div by lia; reflexivity).
+    rewrite Z.mul_comm in Hstep.
+    exact Hstep.
+  }
+  assert (Hq7 : 0 <= value / 72057594037927936 < 256).
+  {
+    split.
+    - apply Z.div_pos; lia.
+    - apply Z.div_lt_upper_bound; lia.
+  }
+  assert (Hstep7 : r7 = q7).
+  {
+    subst q7 r7.
+    rewrite Z.mod_small; lia.
+  }
+  lia.
+Qed.
+
+Lemma ssz_u64_le_bytes_injective :
+  forall value1 value2,
+    0 <= value1 <= uint64_max ->
+    0 <= value2 <= uint64_max ->
+    value1 <> value2 ->
+    ssz_u64_le_bytes value1 <> ssz_u64_le_bytes value2.
+Proof.
+  intros value1 value2 Hrange1 Hrange2 Hneq Hbytes.
+  apply Hneq.
+  pose proof (f_equal ssz_u64_le_decode Hbytes) as Hdecoded.
+  rewrite !ssz_u64_le_decode_encode_roundtrip in Hdecoded by assumption.
   exact Hdecoded.
 Qed.
 
